updating

noActionStacksInIVars/ForkIndependence.v
@@ -1,213 +1,690 @@
-Require Import SfLib.        
-Require Import NonSpec.  
+Require Import SfLib.            
+Require Import NonSpec.   
 Require Import Spec.  
+Require Import Coq.Sets.Ensembles. 
+Require Import erasure. 
 Require Import AST. 
 Require Import hetList. 
 Require Import Coq.Program.Equality. 
 Require Import unspec. 
 Require Import sets. 
-Require Import erasure.  
-Require Import Heap. 
 Require Import classifiedStep. 
-Require Import Coq.Sets.Ensembles. 
 Require Import Coq.Sets.Powerset_facts.  
+Require Import Heap.    
+Require Import IndependenceCommon. 
 
-Theorem EqJMeq : forall (T:Type) (x y:T), x = y -> JMeq x y.
+
+
+Theorem forkFastForward : forall H T H' T' tid s1' s1'' N M M' M'' n E s2 d,
+  decompose M' E (fork M'') -> n = numForks' s2 ->   
+  spec_multistep H (tUnion T (tSingleton(tid,unlocked nil, s2, M')))
+                 H' (tUnion T' (tCouple(tid,unlocked(s1'++[fAct M' E M'' d n]),s2,M)
+                                       (n::tid,locked s1'',nil,N))) ->
+  exists H'' T'',
+    spec_multistep H (tUnion T (tSingleton(tid,unlocked nil,s2,M')))
+                   H'' (tUnion T'' (tCouple(tid,unlocked[fAct M' E M'' d n],s2,fill E (ret unit))
+                                          (n::tid,locked nil,nil,M''))) /\
+    spec_multistep H'' (tUnion T'' (tCouple(tid,unlocked[fAct M' E M'' d n],s2,fill E (ret unit)) (n::tid,locked nil,nil,M'')))
+                   H'(tUnion T' (tCouple(tid,unlocked(s1'++[fAct M' E M'' d n]),s2,M)
+                                       (n::tid,locked s1'',nil,N))) /\
+    spec_multistep H T H'' T''. 
 Proof.
-  intros. subst. auto. Qed. 
-
-Axiom UnionSingletonEq : forall T T' a b, tUnion T (tSingleton a) = tUnion T' (tSingleton b) -> 
-                                          tIn T' a -> T = tUnion (Subtract thread T' a) (tSingleton b).
-
-Axiom uniqueTP : forall T1 T2 t, tIn (tUnion T1 T2) t -> tIn T1 t -> tIn T2 t -> False. 
-
-Ltac cleanup :=
-  match goal with
-      |H: ?x = ?x |- _ => clear H; cleanup
-      |H: ?x = ?y |- _ => inv H
-  end. 
-
-
-Theorem UnionEqTID : forall T T' tid s1 s2 M s1' s2' M',
-                       tUnion T (tSingleton(tid,s1,s2,M)) = tUnion T' (tSingleton(tid,s1',s2',M')) ->
-                       T = T' /\ s1 = s1' /\ s2 = s2' /\ M = M'. 
-Proof. 
-  intros. unfoldSetEq H. assert(tIn (tUnion T (tSingleton(tid,s1,s2,M)))(tid,s1,s2,M)). 
-  apply Union_intror. constructor. copy H.  apply H0 in H. inversion H.  
-  {assert(thread_lookup (tUnion T' (tSingleton(tid,s1',s2',M'))) tid (tid,s1,s2,M)). 
-   econstructor. econstructor. eauto. auto. 
-   assert(thread_lookup (tUnion T' (tSingleton(tid,s1',s2',M'))) tid (tid,s1',s2',M')). 
-   econstructor. apply Union_intror. constructor. auto. eapply uniqueThreadPool in H5; eauto. 
-   inv H5. repeat constructor; auto. eqSets. 
-   {assert(tIn (tUnion T (tSingleton(tid,s1,s2,M))) x). constructor. auto. copy H5. apply H0 in H5. 
-    inversion H5; subst. auto. inv H8. exfalso. eapply uniqueTP; eauto. constructor. }
-   {assert(tIn (tUnion T' (tSingleton(tid,s1,s2,M))) x). constructor. auto. copy H5. 
-    apply H1 in H5. inversion H5; subst. auto. inv H8. exfalso. eapply uniqueTP; eauto. 
-    constructor. }
-  }
-  {subst. inv H3. repeat constructor; auto. eqSets. 
-   {assert(tIn (tUnion T (tSingleton(tid,s1,s2,M))) x). constructor. auto. copy H4. apply H0 in H4. 
-    inversion H4; subst. auto. inv H6. exfalso. eapply uniqueTP; eauto. constructor. }
-   {assert(tIn (tUnion T' (tSingleton(tid,s1,s2,M))) x). constructor. auto. copy H4. 
-    apply H1 in H4. inversion H4; subst. auto. inv H6. exfalso. eapply uniqueTP; eauto. 
-    constructor. }
+  intros. dependent induction H2. 
+  {unfoldTac. rewrite coupleUnion in x. rewrite <- Union_associative in x. 
+   rewrite UnionSwap in x. apply UnionEqTID in x. invertHyp. inv H. invertListNeq. }
+  {copy x. unfoldSetEq H1. copy H. apply specStepSingleton in H1. invertHyp. 
+   assert(tIn (tUnion T0 (tSingleton x0)) x0). apply Union_intror. constructor. 
+   apply H3 in H1. inv H1. 
+   {eapply IHspec_multistep in H0. Focus 4. auto. Focus 2. auto. Focus 2. 
+    apply UnionSingletonEq in x; auto.  
+    rewrite x. unfoldTac. rewrite UnionSwap. auto. invertHyp. exists x1. exists x2.
+    split; auto. apply pullOut in H5. unfoldTac. rewrite H5. rewrite UnionSwap. 
+    econstructor. eapply specStepChangeUnused. eauto. unfoldTac. 
+    rewrite <- UnionSwap. eauto. split. auto. copy H5. apply pullOut in H5. 
+    rewrite H5. econstructor. eapply specStepChangeUnused. eauto. eauto. }
+   {inv H5. apply UnionEqTID in x. invertHyp. clear H1 H5 H7. inversion H; subst. 
+    {unfoldTac; invertHyp; invThreadEq.
+     inv H5; eapply uniqueCtxtDecomp in H0; eauto; invertHyp; solveByInv. }
+    {unfoldTac; invertHyp; invThreadEq. copy d0. eapply uniqueCtxtDecomp in H0; eauto.
+     invertHyp. inv H6. exists h'. exists T. split. econstructor. 
+     eapply SFork; eauto. simpl. constructor. split. simpl in *. assert(d=d0). 
+     apply proof_irrelevance. subst. assumption. constructor. }
+    {unfoldTac; invertHyp; invThreadEq. copy d0; eapply uniqueCtxtDecomp in H0; eauto.
+     invertHyp. inv H7. }
+    {unfoldTac; invertHyp; invThreadEq. copy d0; eapply uniqueCtxtDecomp in H0; eauto.
+     invertHyp. inv H7. }
+    {unfoldTac; invertHyp; invThreadEq. copy d0; eapply uniqueCtxtDecomp in H0; eauto.
+     invertHyp. inv H6. }
+    {unfoldTac; invertHyp; invThreadEq. copy d0; eapply uniqueCtxtDecomp in H0; eauto.
+     invertHyp. inv H6. }
+   }
   }
 Qed.
 
-Theorem specMultiPureThrowout : forall H H' T T' tid s1 s2 M M',
-                                  spec_multistep H (tUnion T (tSingleton(tid,s1,s2,M))) H'
-                                                 (tUnion T' (tSingleton(tid,s1,s2,M'))) ->
-                                  spec_multistep H T H' T'. 
+
+Theorem nonEmptyStack' : forall H H' tid s1 S' s1' a s2 M M' T S T',
+                 spec_multistep H T H' T' -> tIn T (tid,s1,s2,M) ->  tIn T' (tid,s1',s2,M') ->
+                 stackList s1 = S ++ [a] -> stackList s1' = S' -> 
+                 exists s, S' = s ++ [a]. 
 Proof.
-  intros. dependent induction H0. 
-  {apply UnionEqTID in x. invertHyp. constructor. }
-  {copy H. apply specStepSingleton in H. invertHyp. copy x. unfoldSetEq x. 
-   assert(tIn (tUnion T0 (tSingleton x0)) x0). apply Union_intror. constructor. apply H2 in H4. 
-   inversion H4; subst. 
-   {copy H5. apply pullOut in H5. rewrite H5. econstructor. eapply specStepChangeUnused. eauto. 
-    eapply IHspec_multistep; eauto. apply EqJMeq. apply UnionSingletonEq in H; auto.
-    rewrite H. unfoldTac. rewrite Union_associative. rewrite (Union_commutative thread _ t'). 
-    rewrite <- Union_associative. auto. }
-   {inv H5. apply UnionEqTID in H. invertHyp. 
-    inversion H1; subst; try solve[unfoldTac; invertHyp; cleanup; eauto].
-    {unfoldTac; invertHyp; cleanup. eapply monotonicActions with (s1' := s1) in H0.
-     Focus 2. apply Union_intror. apply Couple_l. simpl in H0. Focus 2. 
-     apply Union_intror. constructor. destruct s1; simpl in *; omega. }
-    {unfoldTac; invertHyp; cleanup. eapply monotonicActions in H0. Focus 2. 
-     apply Union_intror; constructor. Focus 2. apply Union_intror. constructor. 
-     simpl in H0. destruct s1; simpl in *; omega. }
-    {unfoldTac; invertHyp; cleanup. eapply monotonicActions in H0. Focus 2. 
-     apply Union_intror; constructor. Focus 2. apply Union_intror. constructor. 
-     simpl in *. destruct s1; simpl in *; omega. }
-    {unfoldTac; invertHyp; cleanup. eapply monotonicActions in H0. Focus 2. 
-     apply Union_intror; constructor. Focus 2. apply Union_intror. constructor. 
-     simpl in *. destruct s1; simpl in *; omega. }
-    {unfoldTac; invertHyp; cleanup. eapply monotonicActions in H0. Focus 2. 
-     apply Union_intror; constructor. Focus 2. apply Union_intror. constructor. 
-     simpl in *. destruct s1; simpl in *; omega. }
+  intros. genDeps{s1';s1;s2;a;M;M';tid;S';S}. induction H0; intros. 
+  {assert(thread_lookup p2 tid (tid,s1,s2,M)). econstructor. eauto. auto. 
+   assert(thread_lookup p2 tid (tid,s1',s2,M')). econstructor. eauto. auto.
+   eapply uniqueThreadPool in H; eauto. invThreadEq. destruct s1; simpl in *; subst; eauto. }
+  {inv H1. 
+   {eapply IHspec_multistep; eauto. constructor. eauto. }
+   {copy H. apply specStepSingleton in H. invertHyp. inv H5. inv H1. 
+    {unfoldTac; invertHyp. inv H. eapply IHspec_multistep; eauto. apply Union_intror. constructor. }
+    {unfoldTac; invertHyp. invThreadEq. eapply IHspec_multistep. apply Union_intror. 
+     constructor. Focus 2. eauto. Focus 2. eauto. destruct s1; simpl in *; subst; simpl;
+     rewrite app_comm_cons; eauto. }
+    {unfoldTac; invertHyp. inv H. eapply IHspec_multistep. apply Union_intror. 
+     constructor. Focus 2. eauto. Focus 2. eauto. destruct s1; simpl in *; subst; 
+     rewrite app_comm_cons; eauto. }
+    {unfoldTac; invertHyp. inv H. eapply IHspec_multistep. apply Union_intror. 
+     constructor. Focus 2. eauto. Focus 2. eauto. destruct s1; simpl in *; subst; 
+     rewrite app_comm_cons; eauto. }
+    {unfoldTac; invertHyp. inv H. eapply IHspec_multistep. apply Union_intror. 
+     constructor. Focus 2. eauto. Focus 2. eauto. destruct s1; simpl in *; subst; 
+     rewrite app_comm_cons; eauto. }
+    {unfoldTac; invertHyp. invThreadEq. eapply IHspec_multistep. apply Union_intror. 
+     constructor. Focus 2. eauto. eauto. Focus 2. eauto. destruct s1; simpl in *; subst; 
+     rewrite app_comm_cons; eauto. }
    }
   }
 Qed.  
 
-Theorem eqUnspec : forall T, T = unspecPoolAux T -> commitPool T. 
+
+Ltac nonEmptyStack'Tac H :=
+  eapply nonEmptyStack' in H;[idtac|apply InL;constructor|apply InL;apply Couple_r|
+                                    rewrite app_nil_l;simpl;auto|auto]. 
+
+
+Theorem forkCatchup : forall H T H' T' x tid' x0 tid s1' s1'' s2 e1 e1' e2 e2' a,
+    eraseTrm s1' e1' x -> eraseTrm s1'' e2' x0 -> 
+    spec_multistep H (tUnion T (tCouple(tid,unlocked[a], s2, e1)
+                                       (tid',locked nil,nil,e2)))
+                   H' (tUnion T' (tCouple(tid,unlocked(s1'++[a]),s2,e1')
+                                         (tid',locked s1'',nil,e2'))) -> 
+    ((
+    exists H'' T'' x0',
+      spec_multistep H (tUnion T (tCouple(tid,unlocked[a],s2,e1)
+                                         (tid',locked nil,nil,e2)))
+                     H'' (tUnion T'' (tCouple(tid,unlocked[a],s2,x)
+                                             (tid',locked nil,nil,x0'))) /\
+      spec_multistep H'' (tUnion T'' (tCouple(tid,unlocked[a],s2,x)
+                                             (tid',locked nil,nil,x0')))
+                 H' (tUnion T' (tCouple(tid,unlocked(s1'++[a]),s2,e1')
+                                         (tid',locked s1'',nil,e2'))) /\
+      spec_multistep H T H'' T'') \/
+     (
+    exists H'' T'' x',
+      spec_multistep H (tUnion T (tCouple(tid,unlocked[a],s2,e1)
+                                         (tid',locked nil,nil,e2)))
+                     H'' (tUnion T'' (tCouple(tid,unlocked[a],s2,x')
+                                             (tid',locked nil,nil,x0))) /\
+      spec_multistep H'' (tUnion T'' (tCouple(tid,unlocked[a],s2,x')
+                                             (tid',locked nil,nil,x0)))
+                 H' (tUnion T' (tCouple(tid,unlocked(s1'++[a]),s2,e1')
+                                         (tid',locked s1'',nil,e2'))) /\
+      spec_multistep H T H'' T'')). 
+Proof.
+  intros. genDeps{x;x0}. dependent induction H2; intros.
+  {unfoldTac. repeat rewrite coupleUnion in x. 
+   repeat rewrite <- Union_associative in x. apply UnionEqTID in x. invertHyp. 
+   inv H3. apply UnionEqTID in H. invertHyp. inv H. destruct s1'; inv H5; try invertListNeq. 
+   inv H0; try invertListNeq. inv H1; try  invertListNeq. left. econstructor. 
+   econstructor. econstructor. split. constructor. split. constructor. constructor. }
+  {copy x. copy H. apply specStepSingleton in H4. invertHyp. copy x. unfoldSetEq x.
+   assert(tIn (tUnion T0 (tSingleton x2)) x2). apply Union_intror. constructor.
+   apply H5 in H7. inv H7. 
+   {eapply IHspec_multistep in H0; eauto. Focus 2. apply UnionSingletonCoupleEq in H3. 
+    rewrite H3. unfoldTac. rewrite UnionSwap. auto. auto. inv H0.  
+    {invertHyp. left. econstructor. econstructor. econstructor. split. takeTStep. 
+     eassumption. split; auto. takeTStep. eassumption. }
+    {invertHyp. right. econstructor. econstructor. econstructor. split. 
+     takeTStep; eauto. split; auto. takeTStep. eauto. }
+   }
+   {inv H8. 
+    {unfoldTac. rewrite coupleUnion in H3. rewrite <- Union_associative in H3.
+     rewrite UnionSwap in H3. apply UnionEqTID in H3. invertHyp. 
+     inv H; unfoldTac; invertHyp; invThreadEq. 
+     {eapply IHspec_multistep in H0. Focus 2. rewrite Union_associative. 
+      rewrite <- coupleUnion. rewrite couple_swap. auto. Focus 2. auto. 
+      Focus 2. eauto. inv H0. 
+      {invertHyp. left. econstructor. econstructor. econstructor. split. 
+       rewrite pullOutL. econstructor. eapply SBasicStep; eauto. unfoldTac. 
+       rewrite <- pullOutL. eassumption. split; auto. }
+      {invertHyp. right. econstructor. econstructor. econstructor. split. 
+       rewrite pullOutL. econstructor. eapply SBasicStep; eauto. unfoldTac. 
+       rewrite <- pullOutL. eassumption. split; auto. }
+     }
+     {copy H2. nonEmptyStackTac H2. invertHyp. apply eraseTrmApp in H0. inv H0. 
+      left. econstructor. econstructor. econstructor. split. constructor. split. 
+      rewrite pullOutL. econstructor. eapply SFork; eauto. eassumption. constructor. }
+     {copy H2. nonEmptyStackTac H2. invertHyp. apply eraseTrmApp in H0. inv H0. 
+      left. econstructor. econstructor. econstructor. split. constructor. split. 
+      rewrite pullOutL. econstructor. eapply SGet; eauto. eassumption. constructor. }
+     {copy H2. nonEmptyStackTac H2. invertHyp. apply eraseTrmApp in H0. inv H0. 
+      left. econstructor. econstructor. econstructor. split. constructor. split. 
+      rewrite pullOutL. econstructor. eapply SPut; eauto. eassumption. constructor. }
+     {copy H2. nonEmptyStackTac H2. invertHyp. apply eraseTrmApp in H0. inv H0. 
+      left. econstructor. econstructor. econstructor. split. constructor. split. 
+      rewrite pullOutL. econstructor. eapply SNew; eauto. eassumption. constructor. }
+     {copy H2. nonEmptyStackTac H2. invertHyp. apply eraseTrmApp in H0. inv H0. 
+      left. econstructor. econstructor. econstructor. split. constructor. split. 
+      rewrite pullOutL. econstructor. eapply SSpec; eauto. eassumption. constructor. }
+    }
+    {unfoldTac. rewrite coupleUnion in H3. rewrite <- Union_associative in H3.
+     apply UnionEqTID in H3. invertHyp. inv H; unfoldTac; invertHyp; invThreadEq. 
+     {eapply IHspec_multistep in H0. Focus 2. rewrite Union_associative. 
+      rewrite <- coupleUnion. auto.  Focus 2. auto. Focus 2. eauto. inv H0. 
+      {invertHyp. left. econstructor. econstructor. econstructor. split. 
+       rewrite pullOutR. econstructor. eapply SBasicStep; eauto. unfoldTac. 
+       rewrite <- pullOutR. eassumption. split; auto. }
+      {invertHyp. right. econstructor. econstructor. econstructor. split. 
+       rewrite pullOutR. econstructor. eapply SBasicStep; eauto. unfoldTac. 
+       rewrite <- pullOutR. eassumption. split; auto. }
+     }
+     {copy H2. simpl in *. nonEmptyStack'Tac H2. invertHyp. simpl in *. subst. 
+      apply eraseTrmApp in H1. inv H1. right. econstructor. econstructor. 
+      econstructor. split. constructor. split; auto. rewrite pullOutR. econstructor. 
+      eapply SFork; eauto. eassumption. constructor. }
+     {copy H2. simpl in *. nonEmptyStack'Tac H2. invertHyp. simpl in *. subst. 
+      apply eraseTrmApp in H1. inv H1. right. econstructor. econstructor. 
+      econstructor. split. constructor. split; auto. rewrite pullOutR. econstructor. 
+      eapply SGet; eauto. eassumption. constructor. }
+     {copy H2. simpl in *. nonEmptyStack'Tac H2. invertHyp. simpl in *. subst. 
+      apply eraseTrmApp in H1. inv H1. right. econstructor. econstructor. 
+      econstructor. split. constructor. split; auto. rewrite pullOutR. econstructor. 
+      eapply SPut; eauto. eassumption. constructor. }
+     {copy H2. simpl in *. nonEmptyStack'Tac H2. invertHyp. simpl in *. subst. 
+      apply eraseTrmApp in H1. inv H1. right. econstructor. econstructor. 
+      econstructor. split. constructor. split; auto. rewrite pullOutR. econstructor. 
+      eapply SNew; eauto. eassumption. constructor. }
+     {copy H2. simpl in *. nonEmptyStack'Tac H2. invertHyp. simpl in *. subst. 
+      apply eraseTrmApp in H1. inv H1. right. econstructor. econstructor. 
+      econstructor. split. constructor. split; auto. rewrite pullOutR. econstructor. 
+      eapply SSpec; eauto. eassumption. constructor. }
+    }
+   }
+  }
+Qed. 
+
+Theorem pureStepsDiffHeap : forall H H' tid s1 s2 M M',
+                              spec_multistep H (tSingleton(tid,s1,s2,M)) H (tSingleton(tid,s1,s2,M')) ->
+                              spec_multistep H' (tSingleton(tid,s1,s2,M)) H' (tSingleton(tid,s1,s2,M')).
 Proof. 
-  intros. unfold commitPool. intros. unfoldSetEq H. apply H1 in H0. inv H0. inv H3; inv H4; auto. 
+  intros. dependent induction H0; unfoldTac. 
+  {invertHyp. invThreadEq. constructor. }
+  {copy H. apply specStepSingleton in H1. invertHyp.  copy x. apply UnionEqSingleton in x. 
+   subst. rewrite <- union_empty_l at 1. inv H; unfoldTac; invertHyp; invThreadEq. 
+   {econstructor. eapply SBasicStep; eauto. unfoldTac. rewrite union_empty_l. 
+    eapply IHspec_multistep; eauto. rewrite <- union_empty_l in H1. 
+    apply UnionEqTID in H1. invertHyp. rewrite union_empty_l. auto. }
+   {eapply monotonicActions in H0. Focus 2. apply InL. constructor. 
+    Focus 2. constructor. destruct s1; simpl in *; omega. }
+   {eapply monotonicActions in H0. Focus 2. apply InL. constructor. 
+    Focus 2. constructor. destruct s1; simpl in *; omega. }
+   {eapply monotonicActions in H0. Focus 2. apply InL. constructor. 
+    Focus 2. constructor. destruct s1; simpl in *; omega. }
+   {eapply monotonicActions in H0. Focus 2. apply InL. constructor. 
+    Focus 2. constructor. destruct s1; simpl in *; omega. }
+   {eapply monotonicActions in H0. Focus 2. apply InL. constructor. 
+    Focus 2. constructor. destruct s1; simpl in *; omega. }
+  }
 Qed. 
 
-Theorem unspecUnlocked : forall tid s1 s2 M t', 
-                   unspecThread (tid,unlocked s1,s2,M) t' ->
-                   exists M',  t' = tSingleton (tid, unlocked nil, s2, M'). 
-Proof.
-  intros. inv H; eauto. 
-Qed. 
-
-
-Ltac eqIn H :=  unfoldTac; 
-  match type of H with
-    | forall x, In ?X (Union ?X ?T (Singleton ?X ?t)) x -> ?z => 
-            assert(In X (Union X T (Singleton X t)) t) by (apply Union_intror; constructor)
-  end. 
-            
-
-Theorem specStepDiffUnused : forall H T H' T' t t',
-                               spec_step H T t H' T t' ->
-                               spec_step H T' t H' T' t'. 
-Proof.
-  intros. inv H0; auto. 
-  {eapply SGet; eauto. }{eapply SPut; eauto. }
-Qed. 
-
-Theorem decomposeNeq : forall M E E' e e', decompose M E e -> decompose M E' e' -> e <> e' ->
-                                           False. 
-Proof.
-  intros. eapply uniqueCtxtDecomp in H; eauto. invertHyp. apply H1. auto.
-Qed. 
-
-Ltac invert := 
-  match goal with
-    |H:?x = ?x |- _ => clear H; invert
-    |H:?x = ?y |- _ => inv H; subst; match goal with
-                                       |H':?x = ?y |- _ => fail
-                                       |_ => idtac
-                                     end 
-  end. 
-
-Theorem forkInd' : forall M M' M'' E N N' h h' T T' s1 s1' s2 d tid,
-      spec_multistep h (tUnion T (tCouple(tid,unlocked[fAct M' E N d], s2, M)
-                                         (1::tid,locked nil, nil, N)))
-                     h' (tUnion T' (tCouple(tid,unlocked(s1++[fAct M' E N d]), s2, M'')
-                                           (1::tid,locked s1', nil, N'))) ->
-      exists h'' T'',
-      spec_multistep h (tUnion T (tCouple(tid,unlocked[fAct M' E N d], s2, M)
-                                         (1::tid,locked nil, nil, N)))
-                     h'' (tUnion T'' (unspecPoolAux(tCouple (tid,unlocked s1,s2,M'')
-                                                            (1::tid,locked s1', nil, N')))) /\
-      spec_multistep h'' (tUnion T''(unspecPoolAux(tCouple (tid,unlocked s1,s2,M'')
-                                                            (1::tid,locked s1', nil, N'))))
-                     h' (tUnion T' (tCouple(tid,unlocked(s1++[fAct M' E N d]), s2, M'')
-                                           (1::tid,locked s1', nil, N'))). 
-Admitted. 
-
-Theorem forkInd : forall H H' T T' tid M M' M'' N s1 s1' s2 E d,
-                    spec_multistep H (tUnion T (tSingleton(tid, unlocked [], s2, M'))) H'
-                                   (tUnion T' (tCouple(tid, unlocked(s1 ++ [fAct M' E M'' d]), s2, M)
-                                                      (1 :: tid, locked s1', nil, N))) ->
-                    spec_multistep H (tUnion T (unspecPoolAux (tCouple (tid,unlocked s1,fAct M' E M'' d::s2, M)
-                                                                       (1::tid,unlocked s1', nil, N))))
-                                   H' (tUnion T' (tCouple(tid,unlocked s1,fAct M' E M'' d::s2, M)
-                                                         (1::tid,unlocked s1', nil, N))).
+Theorem ind1 : forall H H' T T' tid s1 s2 M M',
+                spec_multistep H (tUnion T(tSingleton(tid,s1,s2,M))) 
+                               H' (tUnion T'(tSingleton(tid,s1,s2,M'))) -> 
+                spec_multistep H (tSingleton(tid,s1,s2,M))
+                               H (tSingleton(tid,s1,s2,M')).
 Proof.
   intros. dependent induction H0. 
-  {unfoldTac. rewrite couple_swap in x. rewrite coupleUnion in x. 
-   rewrite <- Union_associative in x. apply UnionEqTID in x. invertHyp. inv H. invertListNeq. }
-  {copy H. apply specStepSingleton in H1. invertHyp. copy x. unfoldSetEq x. eqIn H2. 
-   apply H2 in H4. inversion H4; subst. 
-   {copy H5. apply pullOut in H5. rewrite Union_commutative. rewrite H5. rewrite <- Union_associative. 
-    econstructor. eapply specStepDiffUnused. eauto. unfoldTac. rewrite Union_associative.  
-    rewrite (Union_commutative thread _ t'). rewrite Union_commutative.
-    eapply IHspec_multistep; eauto. apply UnionSingletonEq in H1; auto. rewrite H1. 
-    apply EqJMeq. unfoldTac. rewrite Union_associative. rewrite (Union_commutative thread t').
-    rewrite Union_associative. rewrite (Union_commutative thread t'). auto. }
-   {inv H5. apply UnionEqTID in H1. invertHyp. cleanup. inversion H; subst; try solve[
-     unfoldTac; invertHyp; invert; 
-     match goal with
-       |H:decompose ?M ?E ?e,H':decompose ?M ?E' ?e' |- _ => 
-        assert(CONTRA:e <> e') by introsInv
-     end; eapply decomposeNeq in CONTRA; eauto; contradiction].                                                   
-    {inv H5; unfoldTac; invertHyp; inv H1; 
-     match goal with
-       |H:decompose ?M ?E ?e,H':decompose ?M ?E' ?e' |- _ => 
-        assert(CONTRA:e <> e') by introsInv
-     end; eapply decomposeNeq in CONTRA; eauto; contradiction. }
-    {unfoldTac; invertHyp. invert. simpl in *. copy d; copy d0. eapply uniqueCtxtDecomp in H1; eauto.  
-     invertHyp. inv H7. assert(d=d0) by apply proof_irrelevance. subst. apply forkInd' in H0. 
-     invertHyp. 
+  {apply UnionEqTID in x. invertHyp. constructor. }
+  {startIndCase. eqIn H1. inv H2. 
+   {eapply pureStepsDiffHeap with (H:=h'). eapply IHspec_multistep; eauto. 
+    proveUnionEq x. }
+   {inv H4. rewrite <- union_empty_l at 1. inv H; unfoldTac; invertHyp; invThreadEq. 
+    {econstructor. eapply SBasicStep; eauto. unfoldTac. rewrite union_empty_l. 
+     eapply IHspec_multistep; eauto. }
+    {eapply monotonicActions in H0. Focus 2. apply InL. constructor. Focus 2. 
+     apply InL. constructor. destruct s1; simpl in *; omega. }
+    {eapply monotonicActions in H0. Focus 2. apply InL. constructor. Focus 2. 
+     apply InL. constructor. destruct s1; simpl in *; omega. }
+    {eapply monotonicActions in H0. Focus 2. apply InL. constructor. Focus 2. 
+     apply InL. constructor. destruct s1; simpl in *; omega. }
+    {eapply monotonicActions in H0. Focus 2. apply InL. constructor. Focus 2. 
+     apply InL. constructor. destruct s1; simpl in *; omega. }
+    {eapply monotonicActions in H0. Focus 2. apply InL. constructor. Focus 2. 
+     apply InL. constructor. destruct s1; simpl in *; omega. }
+   }
+  }
+Qed. 
 
-
-
-apply EqJMeq. fold tUnion. unfoldTac. 
-    rewrite (Union_commutative thread t'). rewrite Union_associative. eapply UnionSingletonEq. 
-
-    
-
-Admitted. 
-(*
-Theorem forkInd'' : forall H N TID s2 M E d T T' s,
-                    spec_multistep (unspecHeap H)
-                                   (tUnion T (unspecPoolAux(tSingleton (TID,unlocked(s++[fAct M E N d]),s2,M)))) H
-                                   (tUnion T' (tSingleton(TID,unlocked(s++[fAct M E N d]), s2, M))) ->
-                    spec_multistep (unspecHeap H) 
-                                   (tUnion T (unspecPoolAux(tSingleton(TID,unlocked s,fAct M E N d::s2,M))))
-                                   H (tUnion T' (tSingleton(TID,unlocked s,fAct M E N d::s2,M))).
+Theorem ind2 : forall H H' T T' tid s1 s2 M M',
+                spec_multistep H (tUnion T(tSingleton(tid,s1,s2,M))) 
+                               H' (tUnion T'(tSingleton(tid,s1,s2,M'))) -> 
+                spec_multistep H T H' T'. 
 Proof.
-  intros. erewrite unspecSingleton in H0. Focus 2. unspecThreadTac. auto.  
-  assert(exists t', unspecThread(TID,unlocked s,fAct M E N d::s2, M) t'). apply unspecThreadTotal. 
-  invertHyp. copy H2. apply unspecUnlocked in H2. invertHyp. erewrite unspecSingleton; eauto. 
-  
+  intros. dependent induction H0. 
+  {apply UnionEqTID in x. invertHyp. constructor. }
+  {startIndCase. eqIn H1. inv H2. 
+   {takeTStep. eapply IHspec_multistep; eauto. proveUnionEq x. rewrite H4. solveSet. }
+   {inv H4. apply UnionEqTID in x. invertHyp. inv H; unfoldTac; invertHyp; invThreadEq. 
+    {eauto. }
+    {eapply monotonicActions in H0. Focus 2. apply InL. constructor. Focus 2. 
+     apply InL. constructor. destruct s1; simpl in *; omega. }
+    {eapply monotonicActions in H0. Focus 2. apply InL. constructor. Focus 2. 
+     apply InL. constructor. destruct s1; simpl in *; omega. }
+    {eapply monotonicActions in H0. Focus 2. apply InL. constructor. Focus 2. 
+     apply InL. constructor. destruct s1; simpl in *; omega. }
+    {eapply monotonicActions in H0. Focus 2. apply InL. constructor. Focus 2. 
+     apply InL. constructor. destruct s1; simpl in *; omega. }
+    {eapply monotonicActions in H0. Focus 2. apply InL. constructor. Focus 2. 
+     apply InL. constructor. destruct s1; simpl in *; omega. }
+   }
+  }
+Qed. 
+
+Theorem ind : forall H H' T T' tid s1 s2 M H'' T''  M' s1' M'' ,
+                spec_multistep H (tUnion T(tSingleton(tid,s1,s2,M))) 
+                               H' (tUnion T'(tSingleton(tid,s1,s2,M'))) -> 
+                spec_multistep H' (tUnion T'(tSingleton(tid,s1,s2,M'))) 
+                               H'' (tUnion T''(tSingleton(tid,s1',s2,M''))) -> 
+                spec_multistep H (tUnion T(tSingleton(tid,s1,s2,M)))
+                               H(tUnion T(tSingleton(tid,s1,s2,M'))) /\
+                spec_multistep H(tUnion T(tSingleton(tid,s1,s2,M')))
+                               H'' (tUnion T'' (tSingleton(tid,s1',s2,M''))). 
+Proof.
+  intros. split. 
+  {unfoldTac. rewrite Union_commutative. rewrite (Union_commutative thread T). 
+   rewrite spec_multi_unused. eapply ind1; eauto. }
+  {eapply spec_multi_trans. rewrite spec_multi_unused. eapply ind2; eauto. assumption. }
+Qed. 
+
+
+Ltac nonEmptyStack'Tac2 H :=
+  eapply nonEmptyStack' in H;[idtac|apply InL;constructor|apply InL;constructor|
+                                    rewrite app_nil_l;simpl;auto|auto]. 
+
+Theorem forkCatchupR : forall H T H' T' S S' tid s1 M M' M'' s2,
+          stackList S = nil -> stackList S' = s1 -> eraseTrm s1 M' M'' ->
+          spec_multistep H (tUnion T(tSingleton(tid,S,s2,M)))
+                         H'(tUnion T'(tSingleton(tid,S',s2,M'))) -> 
+          exists H'' T'', 
+            spec_multistep H  (tUnion T(tSingleton(tid,S,s2,M)))
+                           H'' (tUnion T''(tSingleton(tid,S,s2,M''))) /\
+            spec_multistep H'' (tUnion T''(tSingleton(tid,S,s2,M''))) 
+                           H'(tUnion T'(tSingleton(tid,S',s2,M'))).
+Proof.
+  intros. dependent induction H3. 
+  {apply UnionEqTID in x. invertHyp. destruct S'; simpl in *; subst; 
+   inv H2; try invertListNeq; repeat econstructor. }
+  {startIndCase. eqIn H1. inv H4. 
+   {eapply IHspec_multistep in H0; eauto. Focus 2. proveUnionEq x. invertHyp. 
+    econstructor. econstructor. split. takeTStep. eauto. eauto. }
+   {inv H6. apply UnionEqTID in x. invertHyp. inversion H; unfoldTac; invertHyp; invThreadEq. 
+    {eapply IHspec_multistep in H0. Focus 2. eauto. Focus 2. auto. Focus 2. 
+     auto. invertHyp. econstructor. econstructor. split. econstructor. 
+     eapply SBasicStep; eauto. eauto. eauto. }
+    {copy H3. nonEmptyStack'Tac2 H3. Focus 2. destruct S; simpl in *; subst; auto. 
+     invertHyp. rewrite H9 in H2. apply eraseTrmApp in H2. 
+     inv H2. econstructor; econstructor. split. constructor. econstructor. 
+     eapply SFork; eauto. eassumption. }
+    {copy H3. nonEmptyStack'Tac2 H3. Focus 2. destruct S; simpl in *; subst; auto. 
+     invertHyp. rewrite H10 in H2. apply eraseTrmApp in H2. 
+     inv H2. econstructor; econstructor. split. constructor. econstructor. 
+     eapply SGet; eauto. eassumption. }
+    {copy H3. nonEmptyStack'Tac2 H3. Focus 2. destruct S; simpl in *; subst; auto. 
+     invertHyp. rewrite H10 in H2. apply eraseTrmApp in H2. 
+     inv H2. econstructor; econstructor. split. constructor. econstructor. 
+     eapply SPut; eauto. eassumption. }
+    {copy H3. nonEmptyStack'Tac2 H3. Focus 2. destruct S; simpl in *; subst; auto. 
+     invertHyp. rewrite H9 in H2. apply eraseTrmApp in H2. 
+     inv H2. econstructor; econstructor. split. constructor. econstructor. 
+     eapply SNew; eauto. eassumption. }
+    {copy H3. nonEmptyStack'Tac2 H3. Focus 2. destruct S; simpl in *; subst; auto. 
+     invertHyp. rewrite H9 in H2. apply eraseTrmApp in H2. 
+     inv H2. econstructor; econstructor. split. constructor. econstructor. 
+     eapply SSpec; eauto. eassumption. }
+   }
+  }
+Qed. 
+
+Theorem forkCatchupL : forall a H T H' T' S S' tid s1 M M' M'' s2,
+          stackList S = [a] -> stackList S' = s1 ++[a] -> eraseTrm s1 M' M'' ->
+          spec_multistep H (tUnion T(tSingleton(tid,S,s2,M)))
+                         H'(tUnion T'(tSingleton(tid,S',s2,M'))) -> 
+          exists H'' T'', 
+            spec_multistep H  (tUnion T(tSingleton(tid,S,s2,M)))
+                           H'' (tUnion T''(tSingleton(tid,S,s2,M''))) /\
+            spec_multistep H'' (tUnion T''(tSingleton(tid,S,s2,M''))) 
+                           H'(tUnion T'(tSingleton(tid,S',s2,M'))).
+Proof.
+  intros. dependent induction H3.  
+  {apply UnionEqTID in x. invertHyp. destruct S'; simpl in *; subst;  
+   destruct s1; inv H0; try invertListNeq; inv H2; try invertListNeq; repeat econstructor. }
+  {startIndCase. eqIn H4. inv H5. 
+   {eapply IHspec_multistep in H0; eauto. Focus 2. proveUnionEq x. invertHyp. 
+    econstructor. econstructor. split. takeTStep. eauto. eauto. }
+   {inv H7. apply UnionEqTID in x. invertHyp. inversion H; unfoldTac; invertHyp; invThreadEq. 
+    {eapply IHspec_multistep in H0. Focus 2. eauto. Focus 2. eauto. Focus 2. 
+     auto. Focus 2. auto. invertHyp. econstructor. econstructor. split. econstructor. 
+     eapply SBasicStep; eauto. eauto. eauto. }
+    {copy H3. nonEmptyStackTac H3. Focus 2. destruct S; simpl in *; subst; auto. 
+     invertHyp. apply eraseTrmApp in H2. inv H2. econstructor; econstructor. split. 
+     constructor. econstructor. eapply SFork; eauto. eassumption. }
+    {copy H3. nonEmptyStackTac H3. Focus 2. destruct S; simpl in *; subst; auto. 
+     invertHyp. apply eraseTrmApp in H2. inv H2. econstructor; econstructor. split. 
+     constructor. econstructor. eapply SGet; eauto. eassumption. }
+    {copy H3. nonEmptyStackTac H3. Focus 2. destruct S; simpl in *; subst; auto. 
+     invertHyp. apply eraseTrmApp in H2. inv H2. econstructor; econstructor. split. 
+     constructor. econstructor. eapply SPut; eauto. eassumption. }
+    {copy H3. nonEmptyStackTac H3. Focus 2. destruct S; simpl in *; subst; auto. 
+     invertHyp. apply eraseTrmApp in H2. inv H2. econstructor; econstructor. split. 
+     constructor. econstructor. eapply SNew; eauto. eassumption. }
+    {copy H3. nonEmptyStackTac H3. Focus 2. destruct S; simpl in *; subst; auto. 
+     invertHyp. apply eraseTrmApp in H2. inv H2. econstructor; econstructor. split. 
+     constructor. econstructor. eapply SSpec; eauto. eassumption. }
+   }
+  }
+Qed. 
+
+Theorem forkCatchup' : forall H T H' T' x x0 tid s1' tid' s1'' a s2 e1 e1' e2 e2',
+    eraseTrm s1' e1' x -> eraseTrm s1'' e2' x0 ->
+    spec_multistep H (tUnion T (tCouple(tid,unlocked[a], s2, e1)
+                                       (tid',locked nil,nil,e2)))
+                   H' (tUnion T' (tCouple(tid,unlocked(s1'++[a]),s2,e1')
+                                         (tid',locked s1'',nil,e2'))) -> 
+      spec_multistep H (tUnion T (tCouple(tid,unlocked[a],s2,e1)
+                                         (tid',locked nil,nil,e2)))
+                     H (tUnion T (tCouple(tid,unlocked[a],s2,x)
+                                             (tid',locked nil,nil,x0))) /\
+      spec_multistep H (tUnion T (tCouple(tid,unlocked[a],s2,x)
+                                             (tid',locked nil,nil,x0)))
+                 H' (tUnion T' (tCouple(tid,unlocked(s1'++[a]),s2,e1')
+                                         (tid',locked s1'',nil,e2'))).
+Proof.
+  intros. copy H2. eapply forkCatchup in H2; eauto. inv H2. 
+  {invertHyp. unfoldTac. flipCouplesIn H2. flipCouplesIn H4. repeat rewrite coupleUnion in *.
+   repeat rewrite <- Union_associative in *. eapply ind in H2; eauto. invertHyp. unfoldTac.
+   rewrite UnionSwap in H7. rewrite Union_associative in H7. rewrite UnionSwap in H7. 
+   rewrite <- Union_associative in H7. eapply forkCatchupR in H7; eauto. invertHyp. 
+   eapply ind in H8; eauto. invertHyp. split. 
+   {rewrite UnionSwap. eapply spec_multi_trans. eassumption. rewrite UnionSwap. 
+    eapply spec_multi_trans. eassumption. constructor. }
+   {eassumption. }
+  }
+  {invertHyp. unfoldTac. repeat rewrite coupleUnion in *. repeat rewrite <- Union_associative in *. 
+   eapply ind in H2; eauto. invertHyp. unfoldTac. rewrite UnionSwap in H7. 
+   rewrite Union_associative in H7. rewrite UnionSwap in H7. rewrite <- Union_associative in H7.
+   eapply forkCatchupL in H7; simpl;eauto. invertHyp. eapply ind in H8; eauto. invertHyp. split. 
+   {eapply spec_multi_trans. eassumption. rewrite UnionSwap. eapply spec_multi_trans. 
+    eassumption. rewrite UnionSwap. constructor. }
+   {rewrite UnionSwap. rewrite Union_associative. rewrite UnionSwap.
+    rewrite <- Union_associative. assumption. }
+  }
+Qed. 
+
+Theorem nonNilLockedStack : forall s1 s2 x M M' tid H H' T T',
+        actionTerm x M' ->
+        spec_multistep H (tUnion T (tSingleton(tid,locked nil,s2, M')))
+                       H' (tUnion T' (tSingleton(tid,locked s1,s2,M))) ->
+        M <> M' -> s1 <> nil. 
+Proof. 
+  intros. dependent induction H1.  
+  {inv H0; apply UnionEqTID in x; invertHyp; inv H; exfalso; apply H2; auto. }
+  {startIndCase. eqIn H3. inv H4. 
+   {eapply IHspec_multistep; eauto. apply UnionSingletonEq in x. rewrite x. 
+    unfoldTac. rewrite UnionSwap. auto. auto. }
+   {inv H6. inv H0. 
+    {inv H; unfoldTac; invertHyp; invThreadEq; try solve[falseDecomp]. 
+     {inv H4; falseDecomp. }
+     {simpl in *. eapply nonEmptyStack' in H1. Focus 2. apply Union_intror. 
+      constructor. Focus 2. apply Union_intror. constructor. invertHyp. Focus 2. 
+      simpl. rewrite app_nil_l. auto. Focus 2. auto. simpl in *. subst. 
+      introsInv. invertListNeq. }
+    }
+    {inv H; unfoldTac; invertHyp; invThreadEq; try solve[falseDecomp]. 
+     {inv H4; falseDecomp. }
+     {simpl in *. eapply nonEmptyStack' in H1. Focus 2. apply Union_intror. 
+      constructor. Focus 2. apply Union_intror. constructor. invertHyp. Focus 2. 
+      simpl. rewrite app_nil_l. auto. Focus 2. auto. simpl in *. subst. 
+      introsInv. invertListNeq. }
+    }
+    {inv H; unfoldTac; invertHyp; invThreadEq; try solve[falseDecomp]. 
+     {inv H4; falseDecomp. }
+     {simpl in *. eapply nonEmptyStack' in H1. Focus 2. apply Union_intror. 
+      constructor. Focus 2. apply Union_intror. constructor. invertHyp. Focus 2. 
+      simpl. rewrite app_nil_l. auto. Focus 2. auto. simpl in *. subst. 
+      introsInv. invertListNeq. }
+    }
+    {inv H; unfoldTac; invertHyp; invThreadEq; try solve[falseDecomp]. 
+     {inv H4; falseDecomp. }
+     {simpl in *. eapply nonEmptyStack' in H1. Focus 2. apply Union_intror. 
+      constructor. Focus 2. apply Union_intror. constructor. invertHyp. Focus 2. 
+      simpl. rewrite app_nil_l. auto. Focus 2. auto. simpl in *. subst. 
+      introsInv. invertListNeq. }
+    }
+    {inv H; unfoldTac; invertHyp; invThreadEq; try solve[falseDecomp]. 
+     {inv H4; falseDecomp. }
+     {simpl in *. eapply nonEmptyStack' in H1. Focus 2. apply Union_intror. 
+      constructor. Focus 2. apply Union_intror. constructor. invertHyp. Focus 2. 
+      simpl. rewrite app_nil_l. auto. Focus 2. auto. simpl in *. subst. 
+      introsInv. invertListNeq. }
+    }
+   }
+  }
+Qed. 
+
+Inductive stackLists : actionStack -> list action -> actionStack -> list action -> Prop :=
+|stacksL : forall s1 s2, stackLists(locked s1) s1 (locked s2) s2
+|stacksU : forall s1 s2, stackLists(unlocked s1) s1 (unlocked s2) s2
+|stacksS : forall s1 s2 N, stackLists(specStack s1 N) s1 (specStack s2 N) s2.  
+
+
+
+Theorem forkSimActStepsLocked : forall H T H' T' H'' T'' tid s a s' x S S' M M',
+      actionTerm a x -> stackLists S s' S' (s++[a]) ->    
+      spec_multistep H'' (tUnion T'' (tSingleton(tid,locked nil,nil,x)))
+                     H (tUnion T(tSingleton(tid,locked s',nil,M))) -> 
+      spec_multistep H (tUnion T(tSingleton(tid,locked s',nil,M)))
+                     H' (tUnion T'(tSingleton(tid,locked(s++[a]),nil,M'))) ->
+      spec_multistep H (tUnion T(tSingleton(tid, S,nil,M)))
+                     H' (tUnion T'(tSingleton(tid,S',nil,M'))). 
+Proof.
+  intros. genDeps{S;S'}. dependent induction H3; intros. 
+  {apply UnionEqTID in x. invertHyp. inv H. inv H1; constructor. }
+  {startIndCase. eqIn H4. inv H5. 
+   {takeTStep. eapply IHspec_multistep; eauto. eapply spec_multi_trans. eassumption. 
+    rewrite H7. rewrite UnionSwap. econstructor. eapply specStepChangeUnused. eauto. 
+    unfoldTac. rewrite <- UnionSwap. rewrite subtractSingle. constructor. 
+    proveUnionEq x. rewrite H7. solveSet. }
+   {inv H7. apply UnionEqTID in x. invertHyp. inversion H; unfoldTac; invertHyp; invThreadEq. 
+    {copy H2. eapply nonNilLockedStack in H2; eauto. destruct s'. exfalso; apply H2. 
+     auto. econstructor. eapply SBasicStep; eauto. inv H1; constructor. 
+     eapply IHspec_multistep; eauto. eapply spec_multi_trans. eassumption. econstructor. 
+     eapply SBasicStep; eauto. constructor. intros c. inv H0; inv H10; falseDecomp. }
+    {econstructor. eapply SFork with(n:=numForks(locked s')); eauto. inv H1; auto.  unfoldTac. 
+     rewrite couple_swap. rewrite coupleUnion. rewrite <- Union_associative.
+     eapply IHspec_multistep; eauto. eapply spec_multi_trans. 
+     eassumption. rewrite Union_associative. rewrite <- coupleUnion. rewrite couple_swap. 
+     econstructor. eapply SFork with(n:=numForks(locked s')); eauto. constructor. 
+     rewrite Union_associative. rewrite <- coupleUnion. rewrite couple_swap. 
+     simpl in *. rewrite plus_0_r. reflexivity. inv H1; constructor. }
+    {econstructor. eapply SGet; eauto. eapply IHspec_multistep; eauto. 
+     eapply spec_multi_trans. eassumption. econstructor. eapply SGet; eauto. constructor. 
+     simpl. auto. inv H1; simpl; constructor. }
+    {econstructor. eapply SPut; eauto. eapply IHspec_multistep; eauto. 
+     eapply spec_multi_trans. eassumption. econstructor. eapply SPut; eauto. constructor. 
+     simpl. auto. inv H1; simpl; constructor. }
+    {econstructor. eapply SNew; eauto. eapply IHspec_multistep; eauto. 
+     eapply spec_multi_trans. eassumption. econstructor. eapply SNew; eauto. constructor. 
+     simpl. auto. inv H1; simpl; constructor. }
+    {econstructor. eapply SSpec; eauto. unfoldTac. rewrite couple_swap. rewrite coupleUnion. 
+     rewrite <- Union_associative. eapply IHspec_multistep; eauto. eapply spec_multi_trans. 
+     eassumption. rewrite Union_associative. rewrite <- coupleUnion. rewrite couple_swap. 
+     econstructor. eapply SSpec; eauto. constructor. rewrite Union_associative. 
+     rewrite <- coupleUnion. rewrite couple_swap. reflexivity. inv H1; constructor. }
+   }
+  }
+Qed. 
+
+Theorem forkSimActStepsUnlocked : forall H T H' T' H'' s2 T'' z b tid s a s' x M M',
+      eraseTrm(s++[a]) z x -> 
+      spec_multistep H'' (tUnion T'' (tSingleton(tid,unlocked [b],s2,x)))
+                     H (tUnion T(tSingleton(tid,unlocked (s'++[b]),s2,M))) -> 
+      spec_multistep H (tUnion T(tSingleton(tid,unlocked (s'++[b]),s2,M)))
+                     H' (tUnion T'(tSingleton(tid,unlocked(s++[a]++[b]),s2,M'))) ->
+      spec_multistep H (tUnion T(tSingleton(tid, unlocked s',b::s2,M)))
+                     H' (tUnion T'(tSingleton(tid,unlocked(s++[a]),b::s2,M'))). 
+Proof.
+  intros. dependent induction H2; intros. 
+  {apply UnionEqTID in x. invertHyp. inv H. replace [a;b] with([a]++[b]) in H4. 
+   rewrite app_assoc in H4. apply app_inv_tail in H4. subst. inv H1; constructor. 
+   auto. }
+  {startIndCase. eqIn H3. inv H4. 
+   {takeTStep. eapply IHspec_multistep; eauto. eapply spec_multi_trans. eassumption. 
+    rewrite H6. rewrite UnionSwap. econstructor. eapply specStepChangeUnused. eauto. 
+    unfoldTac. rewrite <- UnionSwap. rewrite subtractSingle. constructor. 
+    proveUnionEq x. rewrite H6. solveSet. }
+   {inv H6. apply UnionEqTID in x. invertHyp. inversion H; unfoldTac; invertHyp; invThreadEq. 
+    {copy H1. eapply stackNonNil in H1; eauto. destruct s'. exfalso; apply H1. 
+     auto. econstructor. eapply SBasicStep; eauto. inv H0; constructor. 
+     eapply IHspec_multistep; eauto. eapply spec_multi_trans. eassumption. econstructor. 
+     eapply SBasicStep; eauto. constructor. intros c. apply eraseTrmApp in H0. inv H0; inv H9; falseDecomp. }
+    {econstructor. eapply SFork with(n:=plus (numForks(unlocked(s'++[b])))(numForks' s2)); eauto.
+     simpl. rewrite numForksDistribute. simpl. destruct b; rewrite <- plus_assoc; simpl; auto. 
+     unfoldTac. rewrite couple_swap. rewrite coupleUnion. 
+     rewrite <- Union_associative. eapply IHspec_multistep; eauto. eapply spec_multi_trans. 
+     eassumption. rewrite Union_associative. rewrite <- coupleUnion. rewrite couple_swap. 
+     econstructor. eapply SFork with(n:=plus (numForks(unlocked(s'++[b])))(numForks' s2)); eauto. 
+     simpl. constructor.  rewrite Union_associative. rewrite <- coupleUnion. rewrite couple_swap. 
+     simpl in *. reflexivity. }
+    {econstructor. eapply SGet; eauto. eapply IHspec_multistep; eauto. 
+     eapply spec_multi_trans. eassumption. econstructor. eapply SGet; eauto. constructor. 
+     simpl. auto. }
+    {econstructor. eapply SPut; eauto. eapply IHspec_multistep; eauto. 
+     eapply spec_multi_trans. eassumption. econstructor. eapply SPut; eauto. constructor. 
+     simpl. auto. }
+    {econstructor. eapply SNew; eauto. eapply IHspec_multistep; eauto. 
+     eapply spec_multi_trans. eassumption. econstructor. eapply SNew; eauto. constructor. 
+     simpl. auto. }
+    {econstructor. eapply SSpec; eauto. unfoldTac. rewrite couple_swap. rewrite coupleUnion. 
+     rewrite <- Union_associative. eapply IHspec_multistep; eauto. eapply spec_multi_trans. 
+     eassumption. rewrite Union_associative. rewrite <- coupleUnion. rewrite couple_swap. 
+     econstructor. eapply SSpec; eauto. constructor. rewrite Union_associative. 
+     rewrite <- coupleUnion. rewrite couple_swap. reflexivity. }
+   }
+  }
+Qed. 
+
+
+Theorem forkSimActSteps : forall H T H' T' H'' a' T'' z z' tid s a s' s2 S1 S2 S S' M M' tid' b N N' x x',
+      eraseTrm(S1++[a]) z x -> eraseTrm (S2++[a']) z' x' -> stackLists S s' S' (S2++[a']) ->    
+      spec_multistep H'' (tUnion T'' (tCouple(tid,unlocked[b],s2,x)(tid',locked nil,nil,x')))
+                     H (tUnion T(tCouple(tid,unlocked (s++[b]),s2,M)(tid',locked s',nil,N))) -> 
+      spec_multistep H (tUnion T(tCouple(tid,unlocked (s++[b]),s2,M)(tid',locked s',nil,N)))
+                     H' (tUnion T'(tCouple(tid,unlocked(S1++[a]++[b]),s2,M')(tid',locked(S2++[a']),nil,N'))) ->
+      spec_multistep H (tUnion T(tCouple(tid,unlocked s,b::s2,M)(tid',S,nil,N)))
+                     H' (tUnion T'(tCouple(tid,unlocked(S1++[a]),b::s2,M')(tid',S',nil,N'))).
+Proof.
+  intros. genDeps{S;S'}. dependent induction H4; intros. 
+  {unfoldTac. repeat rewrite coupleUnion in *. repeat rewrite <- Union_associative in *. 
+   apply UnionEqTID in x. invertHyp. apply UnionEqTID in H. invertHyp. 
+   inv H. inv H5. replace[a;b] with([a]++[b]) in H8. rewrite app_assoc in H8. 
+   apply app_inj_tail in H8. invertHyp. inv H2; constructor. auto . }
+  {startIndCase. eqIn H5. inv H6. 
+   {copy H8. takeTStep. eapply IHspec_multistep; eauto. eapply spec_multi_trans. eassumption. 
+    clear H6. takeTStep. rewrite subtractSingle. constructor. apply UnionSingletonCoupleEq in x. 
+    rewrite x. unfoldTac. rewrite UnionSwap. auto. auto. }
+   {inv H8. 
+    {unfoldTac. rewrite couple_swap in x. rewrite coupleUnion in x.
+     rewrite <- Union_associative in x. apply UnionEqTID in x. invertHyp. 
+     inversion H; unfoldTac; invertHyp; invThreadEq.  
+     {copy H3. rewrite couple_swap in H3. rewrite coupleUnion in H3. rewrite couple_swap in H3. 
+      rewrite coupleUnion in H3. repeat rewrite <- Union_associative in H3. eapply stackNonNil in H3. 
+      Focus 2. eauto. destruct s. exfalso; apply H3; auto. rewrite pullOutL. econstructor. 
+      eapply SBasicStep; eauto. constructor. unfoldTac. rewrite <- pullOutL.
+      eapply IHspec_multistep; eauto. eapply spec_multi_trans. eassumption. rewrite pullOutL. 
+      econstructor. eapply SBasicStep; eauto. unfoldTac. rewrite <- pullOutL. constructor. 
+      rewrite Union_associative. rewrite <- coupleUnion. rewrite couple_swap. auto. intros c. 
+      subst. apply eraseTrmApp in H0. inv H0; inv H11; falseDecomp. }
+     {rewrite pullOutL. econstructor.
+      eapply SFork with(n:=plus(numForks (unlocked (s ++ [b]))) (numForks' s2)); eauto.  
+      simpl. rewrite numForksDistribute. simpl. destruct b; rewrite <- plus_assoc; auto. 
+      unfoldTac. rewrite <- UnionSwapR. eapply IHspec_multistep; eauto. eapply spec_multi_trans. 
+      eassumption. rewrite pullOutL. econstructor. eapply SFork; eauto. unfoldTac.
+      rewrite <- UnionSwapR. constructor. rewrite <- UnionSwapR. reflexivity. }
+     {rewrite pullOutL. econstructor. eapply SGet; eauto. unfoldTac. rewrite <- pullOutL. 
+      eapply IHspec_multistep; eauto. eapply spec_multi_trans. eassumption. 
+      rewrite pullOutL. econstructor. eapply SGet; eauto. unfoldTac. rewrite <- pullOutL. 
+      constructor. rewrite <- pullOutL. reflexivity. }
+     {rewrite pullOutL. econstructor. eapply SPut; eauto. unfoldTac. rewrite <- pullOutL. 
+      eapply IHspec_multistep; eauto. eapply spec_multi_trans. eassumption. 
+      rewrite pullOutL. econstructor. eapply SPut; eauto. unfoldTac. rewrite <- pullOutL. 
+      constructor. rewrite <- pullOutL. reflexivity. }
+     {rewrite pullOutL. econstructor. eapply SNew; eauto. unfoldTac. rewrite <- pullOutL. 
+      eapply IHspec_multistep; eauto. eapply spec_multi_trans. eassumption. 
+      rewrite pullOutL. econstructor. eapply SNew; eauto. unfoldTac. rewrite <- pullOutL. 
+      constructor. rewrite <- pullOutL. reflexivity. }
+     {rewrite pullOutL. econstructor. eapply SSpec.  unfoldTac. rewrite <- UnionSwapR. 
+      eapply IHspec_multistep; eauto. eapply spec_multi_trans. 
+      eassumption. rewrite pullOutL. econstructor. eapply SSpec; eauto. unfoldTac.
+      rewrite <- UnionSwapR. constructor. rewrite <- UnionSwapR. reflexivity. }
+    }
+    {unfoldTac. rewrite coupleUnion in x. rewrite <- Union_associative in x.
+     apply UnionEqTID in x. invertHyp. inversion H; unfoldTac; invertHyp; invThreadEq.  
+     {copy H3. repeat rewrite coupleUnion in H3. repeat rewrite <- Union_associative in H3.
+      copy H1. apply eraseTrmApp in H1. eapply nonNilLockedStack in H3; eauto. 
+      destruct s'. exfalso; apply H3; auto. rewrite pullOutR. econstructor. 
+      eapply SBasicStep; eauto. inv H2; constructor. unfoldTac. rewrite <- pullOutR.
+      eapply IHspec_multistep; eauto. eapply spec_multi_trans. eassumption. rewrite pullOutR. 
+      econstructor. eapply SBasicStep; eauto. unfoldTac. rewrite <- pullOutR. constructor. 
+      rewrite Union_associative. rewrite <- coupleUnion. auto. intros c. 
+      subst. inv H1; inv H11; falseDecomp. }
+     {rewrite pullOutR. econstructor.
+      eapply SFork with(n:=plus(numForks (locked s')) (numForks' [])); eauto.  
+      simpl. inv H2; simpl; auto. unfoldTac. rewrite <- UnionSwapR. rewrite couple_swap. 
+      eapply IHspec_multistep; eauto. eapply spec_multi_trans. 
+      eassumption. rewrite pullOutR. econstructor. eapply SFork; eauto. unfoldTac.
+      rewrite <- UnionSwapR. rewrite couple_swap. simpl. rewrite plus_0_r. constructor. 
+      rewrite <- UnionSwapR. rewrite couple_swap. simpl. rewrite plus_0_r. reflexivity. 
+      inv H2; simpl; rewrite plus_0_r;  constructor. }
+     {rewrite pullOutR. econstructor. eapply SGet; eauto. unfoldTac. rewrite <- pullOutR. 
+      eapply IHspec_multistep; eauto. eapply spec_multi_trans. eassumption. 
+      rewrite pullOutR. econstructor. eapply SGet; eauto. unfoldTac. rewrite <- pullOutR. 
+      constructor. rewrite <- pullOutR. reflexivity. inv H2; constructor. }
+     {rewrite pullOutR. econstructor. eapply SPut; eauto. unfoldTac. rewrite <- pullOutR. 
+      eapply IHspec_multistep; eauto. eapply spec_multi_trans. eassumption. 
+      rewrite pullOutR. econstructor. eapply SPut; eauto. unfoldTac. rewrite <- pullOutR. 
+      constructor. rewrite <- pullOutR. reflexivity. inv H2; constructor. }
+     {rewrite pullOutR. econstructor. eapply SNew; eauto. unfoldTac. rewrite <- pullOutR. 
+      eapply IHspec_multistep; eauto. eapply spec_multi_trans. eassumption. 
+      rewrite pullOutR. econstructor. eapply SNew; eauto. unfoldTac. rewrite <- pullOutR. 
+      constructor. rewrite <- pullOutR. reflexivity. inv H2; constructor. }
+     {rewrite pullOutR. econstructor. eapply SSpec.  unfoldTac. rewrite <- UnionSwapR. 
+      rewrite couple_swap. eapply IHspec_multistep; eauto. eapply spec_multi_trans. 
+      eassumption. rewrite pullOutR. econstructor. eapply SSpec; eauto. unfoldTac.
+      rewrite <- UnionSwapR. rewrite couple_swap. constructor. 
+      rewrite <- UnionSwapR. rewrite couple_swap. reflexivity. inv H2; constructor. }
+    }
+   }
+  }
+Qed. 
 
 
 
 
 
 
-asdlkfh*)
+
+
+
+
+
+
+
+
