noActionStacksInIVars/Spec.v
@@ -392,11 +392,11 @@ Inductive step : sHeap -> pool -> pool -> config -> Prop :=
              s1 = unlocked(s1' ++ [fAct M' E M'' d n]) -> n = numForks' s2 ->
              step h T (tCouple (tid, s1, s2, M) (n::tid, locked s1'', nil, N)) (OK h T 
                   (tCouple (tid, unlocked s1', fAct M' E M'' d n::s2, M)
-                           (1::tid, unlocked s1'', nil, N)))
-|PopSpec : forall h s1 s1' s1'' s2 s2' t tid M' M N T E d M'', 
+                           (n::tid, unlocked s1'', nil, N)))
+|PopSpec : forall h s1 s1' s1'' s2 t tid M' M N T E d M'', 
              s1 = unlocked (s1' ++ [srAct t E M N d]) -> 
-             step h T (tCouple(tid, s1, s2, M')(2::tid,locked s1'',s2',M''))
-                  (OK h T (tCouple(tid,unlocked s1',srAct t E M N d::s2,M')(2::tid,specStack s1'' N,s2',M'')))
+             step h T (tCouple(tid, s1, s2, M')(2::tid,locked s1'',nil,M''))
+                  (OK h T (tCouple(tid,unlocked s1',srAct t E M N d::s2,M')(2::tid,specStack s1'' N,nil,M'')))
 .
 
 Hint Constructors step. 
