noActionStacksInIVars/stepWF.v
@@ -1,4 +1,4 @@
-Require Import SfLib.              
+Require Import SfLib.                
 Require Import NonSpec.    
 Require Import Spec.  
 Require Import Coq.Sets.Ensembles. 
@@ -15,7 +15,9 @@ Require Import specIndependence.
 Require Import writeIndependence. 
 Require Import IndependenceCommon. 
 Require Import ReadIndependence. 
-Require Import newIndependence. 
+Require Import newIndependence.  
+Require Import ForkIndependence.
+Require Import PopSpecInd. 
 
 Ltac eUnspec :=
   match goal with
@@ -24,7 +26,7 @@ Ltac eUnspec :=
     | H:spec_multistep ?H ?t ?H' (tUnion ?T' (tSingleton ?t')) |- _ =>
         assert(exists t'', unspecThread t' t'') by apply unspecThreadTotal; invertHyp
   end. 
-
+ 
 Ltac rewriteEmpty xs := 
       match xs with
           |HNil => unfold tUnion; try rewrite union_empty_l; try rewrite union_empty_r
@@ -52,63 +54,12 @@ Ltac invertDecomp :=
      eapply uniqueCtxtDecomp in H; eauto; invertHyp
   end. 
 
-Axiom UnionSingletonCoupleEq : forall T T' a b c, 
-                 tUnion T (tSingleton a) = tUnion T' (tCouple b c) -> 
-                 tIn T' a -> T = tUnion (Subtract thread T' a) (tCouple b c).
 
 Axiom CoupleUnionAx : forall T T' t1 t2,
                         tUnion T (tSingleton t1) = tUnion T' (tCouple t1 t2) -> 
                         T = tUnion T' (tSingleton t2).
 
-Ltac actEqTac H :=
-  eapply firstActEq in H;[idtac|apply Union_intror; rewrite app_nil_l; constructor|
-                          apply Union_intror; constructor]. 
 
-Theorem forkFastForward : forall H T H' T' tid s1' s1'' N M M' M'' n E s2 d,
-  decompose M' E (fork M'') -> n = numForks' s2 ->   
-  spec_multistep H (tUnion T (tSingleton(tid,unlocked nil, s2, M')))
-                 H' (tUnion T' (tCouple(tid,unlocked(s1'++[fAct M' E M'' d n]),s2,M)
-                                       (n::tid,locked s1'',nil,N))) ->
-  exists H'' T'',
-    spec_multistep H (tUnion T (tSingleton(tid,unlocked nil,s2,M')))
-                   H'' (tUnion T'' (tCouple(tid,unlocked[fAct M' E M'' d n],s2,fill E (ret unit))
-                                          (n::tid,locked nil,nil,M''))) /\
-    spec_multistep H'' (tUnion T'' (tCouple(tid,unlocked[fAct M' E M'' d n],s2,fill E (ret unit)) (n::tid,locked nil,nil,M'')))
-                   H'(tUnion T' (tCouple(tid,unlocked(s1'++[fAct M' E M'' d n]),s2,M)
-                                       (n::tid,locked s1'',nil,N))) /\
-    spec_multistep H T H'' T''. 
-Proof.
-  intros. dependent induction H2. 
-  {unfoldTac. rewrite coupleUnion in x. rewrite <- Union_associative in x. 
-   rewrite UnionSwap in x. apply UnionEqTID in x. invertHyp. inv H. invertListNeq. }
-  {copy x. unfoldSetEq H1. copy H. apply specStepSingleton in H1. invertHyp. 
-   assert(tIn (tUnion T0 (tSingleton x0)) x0). apply Union_intror. constructor. 
-   apply H3 in H1. inv H1. 
-   {eapply IHspec_multistep in H0. Focus 4. auto. Focus 2. auto. Focus 2. 
-    apply UnionSingletonEq in x; auto.  
-    rewrite x. unfoldTac. rewrite UnionSwap. auto. invertHyp. exists x1. exists x2.
-    split; auto. apply pullOut in H5. unfoldTac. rewrite H5. rewrite UnionSwap. 
-    econstructor. eapply specStepChangeUnused. eauto. unfoldTac. 
-    rewrite <- UnionSwap. eauto. split. auto. copy H5. apply pullOut in H5. 
-    rewrite H5. econstructor. eapply specStepChangeUnused. eauto. eauto. }
-   {inv H5. apply UnionEqTID in x. invertHyp. clear H1 H5 H7. inversion H; subst. 
-    {unfoldTac; invertHyp; invThreadEq.
-     inv H5; eapply uniqueCtxtDecomp in H0; eauto; invertHyp; solveByInv. }
-    {unfoldTac; invertHyp; invThreadEq. copy d0. eapply uniqueCtxtDecomp in H0; eauto.
-     invertHyp. inv H6. exists h'. exists T. split. econstructor. 
-     eapply SFork; eauto. simpl. constructor. split. simpl in *. assert(d=d0). 
-     apply proof_irrelevance. subst. assumption. constructor. }
-    {unfoldTac; invertHyp; invThreadEq. copy d0; eapply uniqueCtxtDecomp in H0; eauto.
-     invertHyp. inv H7. }
-    {unfoldTac; invertHyp; invThreadEq. copy d0; eapply uniqueCtxtDecomp in H0; eauto.
-     invertHyp. inv H7. }
-    {unfoldTac; invertHyp; invThreadEq. copy d0; eapply uniqueCtxtDecomp in H0; eauto.
-     invertHyp. inv H6. }
-    {unfoldTac; invertHyp; invThreadEq. copy d0; eapply uniqueCtxtDecomp in H0; eauto.
-     invertHyp. inv H6. }
-   }
-  }
-Qed.
  
 Theorem appCons : forall (T:Type) x (y:T) z,
                     x ++ [y;z] = (x ++ [y]) ++ [z]. 
@@ -116,131 +67,8 @@ Proof.
   intros. rewrite <- app_assoc. simpl. auto. Qed. 
 
 
-Theorem forkCatchupOneDone : forall H T H' T' s1 x0 tid s1''' s1' s1'' s2 e1 e1' e2 e2' n,
-    stackList s1' = nil -> eraseTrm (stackList s1''') e2' x0 -> n = numForks' s2 -> 
-    spec_multistep H (tUnion T (tCouple(tid,s1, s2, e1)(n::tid,s1',nil,e2)))
-                   H' (tUnion T' (tCouple(tid,s1'',s2,e1')(n::tid,s1''',nil,e2'))) -> 
-    exists H'' T'',
-      spec_multistep H (tUnion T (tCouple(tid,s1,s2,e1)(n::tid,s1',nil,e2)))
-                     H'' (tUnion T'' (tCouple(tid,s1,s2,e1)(n::tid,s1',nil,x0))) /\
-      spec_multistep H'' (tUnion T'' (tCouple(tid,s1,s2,e1)(n::tid,s1',nil,x0)))
-                   H' (tUnion T' (tCouple(tid,s1'',s2,e1')(n::tid,s1''',nil,e2'))) /\
-      spec_multistep H T H'' T''. 
-Proof.
-  intros. dependent induction H3. 
-  {unfoldTac. repeat rewrite coupleUnion in x. 
-   repeat rewrite <- Union_associative in x. apply UnionEqTID in x. invertHyp. 
-   apply UnionEqTID in H. invertHyp. destruct s1'''; 
-   simpl in *; subst; inv H1; try invertListNeq; do 5 econstructor. }
-  {startIndCase. eqIn H2. inv H4. 
-   {eapply IHspec_multistep in H1; eauto. Focus 2. apply UnionSingletonCoupleEq in x.
-    rewrite x. unfoldTac. rewrite UnionSwap. auto. auto. invertHyp. 
-    econstructor. econstructor. split. takeTStep. eassumption. split; auto. 
-    takeTStep. eauto. }
-   {inv H6. 
-    {unfoldTac. rewrite coupleUnion in x. rewrite <- Union_associative in x. 
-     rewrite UnionSwap in x. apply UnionEqTID in x. invertHyp. 
-     inversion H; unfoldTac; invertHyp; invThreadEq. 
-     {eapply IHspec_multistep in H1;[idtac|eauto|eauto|idtac|auto]. Focus 2. 
-      rewrite UnionSwap. rewrite Union_associative. rewrite <- coupleUnion. 
-      auto. invertHyp. econstructor. econstructor. split. 
-      repeat rewrite pullOutL in *. rewrite spec_multi_unused. 
-      rewrite spec_multi_unused in H7. eassumption. split. rewrite pullOutL. 
-      econstructor. eapply SBasicStep; eauto. unfoldTac. rewrite <- pullOutL. 
-      eassumption. eauto. }
-     {eapply IHspec_multistep in H1;[idtac|eauto|eauto|idtac|auto]. Focus 2.
-      rewrite UnionSwap. rewrite pullOutL. rewrite Union_associative. 
-      rewrite <- coupleUnion. auto. invertHyp. econstructor; econstructor;
-      split. 
-
-
-
-Ltac flipCouples :=
-  rewrite couple_swap; rewrite coupleUnion; try flipCouples; rewrite <- coupleUnion. 
-
-Ltac flipCouplesIn H :=
-  rewrite couple_swap in H; rewrite coupleUnion in H; try flipCouplesIn H; rewrite <- coupleUnion in H. 
-
-Theorem forkCatchup : forall H T H' T' x x0 tid s1' s1'' s2 e1 e1' e2 e2' M' M'' n E d,
-    eraseTrm s1' e1' x -> eraseTrm s1'' e2' x0 -> n = numForks' s2 -> 
-    spec_multistep H (tUnion T (tCouple(tid,unlocked[fAct M' E M'' d n], s2, e1)
-                                       (n::tid,locked nil,nil,e2)))
-                   H' (tUnion T' (tCouple(tid,unlocked(s1'++[fAct M' E M'' d n]),s2,e1')
-                                         (n::tid,locked s1'',nil,e2'))) -> 
-    exists H'' T'',
-      spec_multistep H (tUnion T (tCouple(tid,unlocked[fAct M' E M'' d n],s2,e1)
-                                         (n::tid,locked nil,nil,e2)))
-                     H'' (tUnion T'' (tCouple(tid,unlocked[fAct M' E M'' d n],s2,x)
-                                             (n::tid,locked nil,nil,x0))) /\
-      spec_multistep H'' (tUnion T'' (tCouple(tid,unlocked[fAct M' E M'' d n],s2,x)
-                                             (n::tid,locked nil,nil,x0)))
-                 H' (tUnion T' (tCouple(tid,unlocked(s1'++[fAct M' E M'' d n]),s2,e1')
-                                         (n::tid,locked s1'',nil,e2'))) /\
-      spec_multistep H T H'' T''. 
-Proof.
-  intros. genDeps{x;x0}. dependent induction H3; intros.
-  {unfoldTac. repeat rewrite coupleUnion in x. 
-   repeat rewrite <- Union_associative in x. apply UnionEqTID in x. invertHyp. 
-   inv H3. apply UnionEqTID in H. invertHyp. inv H. destruct s1'; inv H5. 
-   inv H0; try invertListNeq. inv H1; try  invertListNeq. exists h. exists T'. 
-   split. constructor. split. constructor. constructor. invertListNeq. }
-  {copy x. copy H. apply specStepSingleton in H4. invertHyp. copy x. unfoldSetEq x.
-   assert(tIn (tUnion T0 (tSingleton x2)) x2). apply Union_intror. constructor.
-   apply H5 in H7. inv H7. 
-   {eapply IHspec_multistep in H0; eauto. invertHyp. exists x. exists x3. 
-    split. copy H8. apply pullOut in H9. rewrite H9. unfoldTac. rewrite UnionSwap. 
-    econstructor. eapply specStepChangeUnused. eauto. unfoldTac. rewrite <- UnionSwap.
-    eauto. split. auto. copy H8. apply pullOut in H9. rewrite H9. econstructor. 
-    eapply specStepChangeUnused. eauto. auto. apply UnionSingletonCoupleEq in H2. 
-    rewrite H2. unfoldTac. rewrite UnionSwap. auto. auto. }
-   {inv H8. 
-    {unfoldTac. rewrite coupleUnion in H2. rewrite <- Union_associative in H2.
-     rewrite UnionSwap in H2. apply UnionEqTID in H2. invertHyp. 
-     inv H; unfoldTac; invertHyp; invThreadEq. 
-     {eapply IHspec_multistep in H0. invertHyp. exists x. exists x2. 
-      split. rewrite coupleUnion. rewrite <- Union_associative. rewrite UnionSwap. 
-      econstructor. eapply SBasicStep. eauto. constructor. unfoldTac. 
-      rewrite <- UnionSwap. rewrite Union_associative. rewrite <- coupleUnion. 
-      eauto. split. eassumption. assumption.  auto. rewrite Union_associative. 
-      rewrite <- coupleUnion. rewrite couple_swap. auto. auto. auto. }
-     {simpl in *. copy H3. nonEmptyStackTac H3. invertHyp. copy H0. 
-      apply eraseTrmApp in H0. inv H0. rewrite UnionSwapR in H. 
-      eapply forkCatchupOneDone; eauto. unfoldTac. rewrite pullOutL. econstructor. eapply SFork; eauto. unfoldTac. rewrite UnionSwapR. eassumption. }
-     {simpl in *. copy H3. nonEmptyStackTac H3. invertHyp. copy H0. apply eraseTrmApp in H0. 
-      inv H0. eapply forkCatchupOneDone; eauto. unfoldTac. rewrite pullOutL. econstructor. 
-      eapply SGet; eauto. unfoldTac. eassumption. }
-     {simpl in *. copy H3. nonEmptyStackTac H3. invertHyp. copy H0. apply eraseTrmApp in H0. 
-      inv H0. eapply forkCatchupOneDone; eauto. unfoldTac. rewrite pullOutL. econstructor. 
-      eapply SPut; eauto. unfoldTac. eassumption. }
-     {simpl in *. copy H3. nonEmptyStackTac H3. invertHyp. copy H0. apply eraseTrmApp in H0. 
-      inv H0. eapply forkCatchupOneDone; eauto. unfoldTac. rewrite pullOutL. econstructor. 
-      eapply SNew; eauto. unfoldTac. eassumption. }
-     {simpl in *. copy H3. nonEmptyStackTac H3. invertHyp. copy H0. apply eraseTrmApp in H0. 
-      inv H0. eapply forkCatchupOneDone; eauto. unfoldTac. rewrite pullOutL. econstructor. 
-      eapply SSpec; eauto. unfoldTac. eassumption. }
-    } 
-    {unfoldTac. rewrite coupleUnion in H2. rewrite <- Union_associative in H2. 
-     apply UnionEqTID in H2. invertHyp. inv H; unfoldTac; invertHyp; invThreadEq. 
-     {eapply IHspec_multistep in H0;[idtac|eauto|eauto|eauto|eauto]. Focus 2. 
-      rewrite Union_associative. rewrite <- coupleUnion. auto. invertHyp. econstructor. 
-      econstructor. split. rewrite pullOutR. econstructor. eapply SBasicStep; eauto. 
-      unfoldTac. rewrite <- pullOutR. eauto. split. eauto. eauto. }
-     {simpl in *. copy H3. rewrite couple_swap in H. eapply monotonicActions in H. 
-      Focus 2. apply InL. apply Couple_r. Focus 2. apply InL. apply Couple_r. simpl in *. 
-      destructLast s1''. simpl in *. omega. invertHyp. apply eraseTrmApp in H1. 
-      inv H1. 
-
-Ltac nonEmptyStackTac H :=
-  try(eapply nonEmptyStack in H;[ idtac
-                                | apply InL; constructor
-                                | solve[solveSet]
-                                | simpl; try rewrite app_nil_l; eauto   
-                                | simpl; eauto]);
-  try(eapply nonEmptyStack in H;[ idtac
-                                | apply InL; apply Couple_r
-                                | solve[solveSet]
-                                | simpl; try rewrite app_nil_l; eauto   
-                                | simpl; eauto]); fail. 
+Ltac monoActs H := 
+  eapply monotonicActions in H;[idtac|apply InL; constructor|apply InL; constructor]. 
 
 
 Theorem listTailEq : forall (T:Type) a (b:T) c d e,
@@ -363,28 +191,81 @@ Proof.
    constructor. auto. }
 Qed. 
 
-Theorem raw_lookupCreatedSpec : forall x H ds t0 N s S,
+Theorem raw_lookupCreatedSpecFull : forall x H ds t0 N s S,
                                   unique ivar_state S H -> 
-                                  (raw_heap_lookup x H = Some(sempty SPEC) \/
-                                  raw_heap_lookup x H = Some(sfull SPEC ds s t0 N)) ->
+                                  raw_heap_lookup x H = Some(sfull SPEC ds s t0 N) ->
                                   raw_heap_lookup x (raw_unspecHeap H) = None. 
 Proof. 
   induction H; intros. 
   {inv H0; inv H1. }
   {simpl in *. destruct a. destruct (beq_nat x i) eqn:eq. 
-   {inv H0. inv H1; inv H0; apply unspecUnique in H7; eapply uniqueLookupNone; eauto;
+   {inv H0. inv H1. apply unspecUnique in H7; eapply uniqueLookupNone; eauto;
     apply beq_nat_true in eq; subst; apply Union_intror; constructor. }
    {inv H0. destruct i0. destruct s0. eauto. simpl. rewrite eq. eauto. 
     destruct s0; eauto. destruct s1; simpl; rewrite eq; eauto. }
   }
 Qed. 
 
-Theorem lookupCreatedSpec : forall x H ds t0 N s,
-                                  (heap_lookup x H = Some(sempty SPEC) \/
-                                  heap_lookup x H = Some(sfull SPEC ds s t0 N)) ->
+Theorem lookupCreatedSpecFull : forall x H ds t0 N s,
+                                  heap_lookup x H = Some(sfull SPEC ds s t0 N) ->
                                   heap_lookup x (unspecHeap H) = None. 
 Proof.
-  intros. destruct H. simpl. eapply raw_lookupCreatedSpec; eauto. 
+  intros. destruct H. simpl. eapply raw_lookupCreatedSpecFull; eauto. 
+Qed. 
+
+Theorem raw_lookupCreatedSpecEmpty : forall x H S,
+                                  unique ivar_state S H -> 
+                                  raw_heap_lookup x H = Some(sempty SPEC) -> 
+                                  raw_heap_lookup x (raw_unspecHeap H) = None. 
+Proof. 
+  induction H; intros. 
+  {inv H0; inv H1. }
+  {simpl in *. destruct a. destruct (beq_nat x i) eqn:eq. 
+   {inv H0. inv H1; apply unspecUnique in H7; eapply uniqueLookupNone; eauto;
+    apply beq_nat_true in eq; subst; apply Union_intror; constructor. }
+   {inv H0. destruct i0. destruct s. eauto. simpl. rewrite eq. eauto. 
+    destruct s; eauto. destruct s0; simpl; rewrite eq; eauto. }
+  }
+Qed. 
+
+Theorem lookupCreatedSpecEmpty : forall x H,
+                                  heap_lookup x H = Some(sempty SPEC) ->
+                                  heap_lookup x (unspecHeap H) = None. 
+Proof.
+  intros. destruct H. simpl. eapply raw_lookupCreatedSpecEmpty; eauto. 
+Qed. 
+
+
+Theorem PopSpecFastForward : forall H T H' T' tid s1' s1'' N M M' M'' N'' E s2 d,
+  decompose M' E (spec M'' N'') -> 
+  spec_multistep H (tUnion T (tSingleton(tid,unlocked nil, s2, M')))
+                 H' (tUnion T' (tCouple(tid,unlocked(s1'++[srAct M' E M'' N'' d]),s2,M)
+                                       (2::tid,locked s1'',nil,N))) ->
+  exists H'' T'',
+    spec_multistep H (tUnion T (tSingleton(tid,unlocked nil,s2,M')))
+                   H'' (tUnion T'' (tCouple(tid,unlocked[srAct M' E M'' N'' d],s2,fill E (specRun M'' N''))
+                                          (2::tid,locked nil,nil,N''))) /\
+    spec_multistep H'' (tUnion T'' (tCouple(tid,unlocked[srAct M' E M'' N'' d],s2,fill E (specRun M'' N'')) 
+                                           (2::tid,locked nil,nil,N'')))
+                   H'(tUnion T' (tCouple(tid,unlocked(s1'++[srAct M' E M'' N'' d]),s2,M)
+                                       (2::tid,locked s1'',nil,N))) /\
+    spec_multistep H T H'' T''. 
+Proof.
+  intros. dependent induction H1. 
+  {unfoldTac. rewrite coupleUnion in x. rewrite <- Union_associative in x. 
+   rewrite UnionSwap in x. apply UnionEqTID in x. invertHyp. inv H. invertListNeq. }
+  {startIndCase. eqIn H2. inv H3. 
+   {eapply IHspec_multistep in H0; eauto. Focus 2. proveUnionEq x. invertHyp. 
+    econstructor. econstructor. split. takeTStep. eassumption. split; eauto. 
+    takeTStep. eauto. }
+   {inv H5. apply UnionEqTID in x. invertHyp. econstructor. econstructor. split. econstructor. 
+    eapply SSpec; eauto. simpl. constructor. split; try constructor. 
+    inv H; unfoldTac; invertHyp; invThreadEq; try solve[falseDecomp]. 
+    {inv H8; falseDecomp. }
+    {simpl in *. copy d0. eapply uniqueCtxtDecomp in H0; eauto. invertHyp. 
+     inv H8. proofsEq d d0. eassumption. }
+   }
+  }
 Qed. 
 
 Theorem stepWF : forall H T t H' t', 
@@ -556,7 +437,7 @@ Proof.
    rewrite unspecUnionComm in *. erewrite unspecSingleton in H4. Focus 2. 
    unspecThreadTac. auto. eraseTrmTac s1' M. erewrite unspecSingleton. Focus 2. 
    apply unspecEraseTrm; eauto. eapply newFastForward in H4; eauto. Focus 2. 
-   eapply lookupCreatedSpec; eauto. invertHyp. eapply spec_multi_trans.
+   eapply lookupCreatedSpecFull; eauto. invertHyp. eapply spec_multi_trans.
    rewrite spec_multi_unused. eassumption. eapply newSimPureStepsFull in H3; eauto. 
    inv H3.  
    {invertHyp. eapply spec_multi_trans. rewrite spec_multi_unused. eassumption. 
@@ -578,7 +459,7 @@ Proof.
    rewrite unspecUnionComm in *. erewrite unspecSingleton in H4. Focus 2. 
    unspecThreadTac. auto. eraseTrmTac s1' M. erewrite unspecSingleton. Focus 2. 
    apply unspecEraseTrm; eauto. eapply newFastForward in H4; eauto. Focus 2. 
-   eapply lookupCreatedSpec; eauto. invertHyp. eapply spec_multi_trans.
+   eapply lookupCreatedSpecEmpty; eauto. invertHyp. eapply spec_multi_trans.
    rewrite spec_multi_unused. eassumption. eapply newSimPureStepsEmpty in H3; eauto. 
    invertHyp. eapply spec_multi_trans. rewrite spec_multi_unused. eassumption. 
    destructLast s1'. 
@@ -594,17 +475,46 @@ Proof.
    apply unspecEraseTrm. eauto. unfoldTac. rewrite union_empty_r in H3. 
    rewrite <- coupleUnion in H3. eapply forkFastForward in H3; eauto. invertHyp.
    eapply spec_multi_trans. erewrite spec_multi_unused. eassumption. 
-   repeat rewrite <- coupleUnion. eapply forkCatchup in H3; eauto. 
-   invertHyp. eapply spec_multi_trans. rewrite spec_multi_unused. eassumption. 
-   
-   
-
-
-
-
-  
-
-
-
-
-aldsfhlasdkjhfasd
+   repeat rewrite <- coupleUnion. eapply forkCatchup' in H3; eauto. invertHyp. 
+   destructLast s1'. 
+   {destructLast s1''. 
+    {inv H2;inv H0; try invertListNeq. rewrite spec_multi_unused. simpl in *.  
+      unfoldTac. rewrite spec_multi_unused in H6. assumption. }
+    {invertHyp. inv H0; try invertListNeq. unfoldTac. flipCouples. flipCouplesIn H6.  
+      repeat rewrite coupleUnion in *. repeat rewrite <- Union_associative in *. 
+      rewrite spec_multi_unused. rewrite spec_multi_unused in H6. apply eraseTrmApp in H2. 
+      eapply forkSimActStepsLocked; eauto. constructor. constructor. }
+   }
+   {invertHyp. destructLast s1''. 
+    {inv H2; try invertListNeq. unfoldTac. repeat rewrite coupleUnion in *. 
+     repeat rewrite <- Union_associative in *. rewrite spec_multi_unused. 
+     rewrite spec_multi_unused in H6. eapply forkSimActStepsUnlocked; eauto. 
+     constructor. rewrite <- app_assoc in H6. simpl in *. auto. }
+    {invertHyp. eapply forkSimActSteps; eauto. constructor. constructor. 
+     rewrite <- app_assoc in H6. simpl in *. assumption. }
+   }
+  }
+  {inv H0. inv H2. econstructor; eauto. unfoldTac. rewrite coupleUnion in *.  
+   repeat rewrite unspecUnionComm in *. eraseTrmTac s1' M'. rUnspecAll. 
+   Focus 2. unspecThreadTac; eauto. Focus 3. unspecThreadTac; eauto. 
+   Focus 2. apply unspecEraseTrm; eauto. eraseTrmTac s1'' M''. rUnspecAll. 
+   unfoldTac. rewrite union_empty_r in H3. rewrite <- coupleUnion in H3. 
+   eapply PopSpecFastForward in H3; eauto. invertHyp.
+   eapply spec_multi_trans. erewrite spec_multi_unused. eassumption. 
+   repeat rewrite <- coupleUnion. unfoldTac. flipCouplesIn H3. 
+   repeat rewrite coupleUnion in H3. repeat rewrite <- Union_associative in H3. 
+   eapply forkCatchupL in H3; eauto. Focus 2. simpl. auto. Focus 2. simpl. auto. 
+   invertHyp. eapply ind in H6; eauto. invertHyp. clear H3. unfoldTac. 
+   rewrite Union_associative in H7. rewrite <- coupleUnion in H7. flipCouplesIn H7. 
+   destructLast s1'. 
+   {inv H0; try invertListNeq. rewrite couple_swap in H7.  rewrite coupleUnion in H7. 
+    rewrite <- Union_associative in H7. rewrite spec_multi_unused in H7. flipCouples.  
+    repeat rewrite coupleUnion. repeat rewrite <- Union_associative. rewrite spec_multi_unused. 
+    apply simSpecStackSteps. assumption. }
+   {invertHyp. eapply specSimActSteps; eauto. constructor. rewrite <- app_assoc in H7. 
+    simpl in *. rewrite Union_associative in H7. rewrite <- coupleUnion in H7. 
+    rewrite couple_swap in H7. flipCouplesIn H7. assumption. }
+  }
+  Grab Existential Variables. eapply lookupCreatedSpecEmpty; eauto. 
+  eapply lookupCreatedSpecFull; eauto. 
+Qed. 
